Cslib/Computability/LambdaCalculus/LocallyNameless/Fsub/Properties.lean
@@ -1,0 +1,52 @@
+/-
+Copyright (c) 2025 Chris Henson. All rights reserved.
+Released under Apache 2.0 license as described in the file LICENSE.
+Authors: Chris Henson
+-/
+
+import Cslib.Computability.LambdaCalculus.LocallyNameless.Fsub.Basic
+
+/-! # λ-calculus
+
+The λ-calculus with polymorphism and subtyping, with a locally nameless representation of syntax.
+
+## References
+
+* [A. Chargueraud, *The Locally Nameless Representation*][Chargueraud2012]
+* See also <https://www.cis.upenn.edu/~plclub/popl08-tutorial/code/>, from which
+  this is adapted
+
+-/
+
+universe u
+
+variable {Var : Type u} [HasFresh Var] [DecidableEq Var]
+
+namespace LambdaCalculus.LocallyNameless.Fsub
+
+attribute [simp] Ty.open_tt_rec
+
+lemma Ty.open_tt_rec_type_aux : forall (T : Ty Var) j V i U,
+  i ≠ j ->
+  open_tt_rec j V T = open_tt_rec i U (open_tt_rec j V T) ->
+  T = open_tt_rec i U T := by
+  intros T
+  induction T <;> intros j V i U neq H
+  case bvar i' => 
+    by_cases eq : i = i' <;> [subst eq; skip] <;> simp_all only [neq.symm, open_tt_rec, reduceIte]
+  case arrow l r ih_l ih_r => 
+    simp only [open_tt_rec, arrow.injEq] at *
+    have ⟨Hl, Hr⟩ := H 
+    exact ⟨ih_l j V i U neq Hl, ih_r j V i U neq Hr⟩
+  case all l r ih_l ih_r =>
+    simp only [open_tt_rec, all.injEq] at *
+    have ⟨Hl, Hr⟩ := H 
+    refine ⟨ih_l j V i U neq Hl, ih_r (j + 1) V (i + 1) U (by grind) Hr⟩
+  case sum l r ih_l ih_r => 
+    simp only [open_tt_rec, sum.injEq] at *
+    have ⟨Hl, Hr⟩ := H 
+    exact ⟨ih_l j V i U neq Hl, ih_r j V i U neq Hr⟩
+  case top => simp only [open_tt_rec]
+  case fvar => simp only [open_tt_rec]
+
+end LambdaCalculus.LocallyNameless.Fsub
